added ty_of_sat'_safe lemma

thys/MFODL_Monitor_Devel/Type_Soundness.thy
@@ -93,7 +93,7 @@ fun sat' :: "Formula.trace \<Rightarrow> (Formula.name \<rightharpoonup> nat \<R
      | Some X \<Rightarrow> map (eval_trm' v) ts \<in> X i)"
 | "sat' \<sigma> V v i (Formula.Let p \<phi> \<psi>) =
     sat' \<sigma> (V(p \<mapsto> \<lambda>i. {v. length v = Formula.nfv \<phi> \<and> sat' \<sigma> V v i \<phi>})) v i \<psi>"
-| "sat' \<sigma> V v i (Formula.Eq t1 t2) = undef_eq (eval_trm' v t1) (eval_trm' v t2)"
+| "sat' \<sigma> V v i (Formula.Eq t1 t2) =  (eval_trm' v t1 = eval_trm' v t2)"
 | "sat' \<sigma> V v i (Formula.Less t1 t2) = undef_less (eval_trm' v t1) (eval_trm' v t2)"
 | "sat' \<sigma> V v i (Formula.LessEq t1 t2) = undef_less_eq (eval_trm' v t1) (eval_trm' v t2)"
 | "sat' \<sigma> V v i (Formula.Neg \<phi>) = (\<not> sat' \<sigma> V v i \<phi>)"
@@ -140,6 +140,413 @@ lemma eval_trm_sound:
 lemma nfv_exists: " Formula.nfv \<phi> \<le> Suc (Formula.nfv (Formula.Exists t \<phi>))"
    apply (auto simp add: Formula.nfv_def fvi_Suc) 
   by (metis Max.coboundedI finite_fvi finite_imageI finite_insert fvi_Suc imageI insertCI list_decode.cases)
+
+lemma match_sat'_fv: assumes "safe_regex temp Strict r"
+    "Regex.match (sat' \<sigma> V v) r j i"
+    "x \<in> fv (formula.MatchP I r) \<or> x \<in>fv (formula.MatchF I r)"
+  shows "\<exists>\<phi>\<in>atms r. \<exists>k. sat' \<sigma> V v k \<phi> \<and> x \<in> fv \<phi>"
+  using assms
+  proof (induction r arbitrary:i j)
+
+    case (Plus r1 r2)
+  moreover obtain k where "\<exists>j. Regex.match (sat' \<sigma> V v) r1 j k \<or>  Regex.match (sat' \<sigma> V v) r2 j k" using  Plus.prems(2)  by auto
+  moreover {
+    assume assm: "\<exists>j. Regex.match (sat' \<sigma> V v) r1 j k"
+    then have ?case using Plus.prems(1,3) Plus.IH(1)  by (fastforce simp add: atms_def) 
+  } moreover {
+    assume assm: "\<exists>j. Regex.match (sat' \<sigma> V v) r2 j k"
+    from this have ?case using Plus.prems(1,3) Plus.IH(2) by (fastforce simp add: atms_def)
+  }
+  ultimately show ?case by auto
+next
+  case (Times r1 r2)
+  then show ?case  using Times.prems match_le Times.IH  by (cases temp) fastforce+
+qed  auto
+
+
+
+lemma ty_of_sat'_safe: "safe_formula \<phi> \<Longrightarrow> S, E \<turnstile> \<phi> \<Longrightarrow> wty_envs S \<sigma> V \<Longrightarrow> 
+  sat' \<sigma> V v i \<phi> \<Longrightarrow> x \<in> Formula.fv \<phi> \<Longrightarrow> Formula.nfv \<phi> \<le> length v \<Longrightarrow> ty_of (v ! x) = E x"
+proof (induction arbitrary: S E V v i x rule: safe_formula_induct)
+  case (Eq_Const c d)
+  then show ?case by auto
+next
+  case (Eq_Var1 c xa)
+   case (Eq_Var1 c xa)
+  from Eq_Var1.prems(1) obtain t where 
+" E \<turnstile> (trm.Const c) :: t" and "E \<turnstile> (trm.Var xa) :: t"
+    by cases
+  from Eq_Var1(4)  have "x = xa" by auto
+  from this `E \<turnstile> (trm.Var xa) :: t` have "E x = t" using  wty_trm.cases by fastforce
+  from this Eq_Var1 ` E \<turnstile> (trm.Const c) :: t` show ?case
+    by (metis \<open>x = xa\<close> empty_iff eval_trm'.simps(1) fvi_trm.simps(2) sat'.simps(3) eval_trm_sound ty_of_eval_trm)
+
+next
+  case (Eq_Var2 c xa)
+    from Eq_Var2.prems(1) obtain t where 
+" E \<turnstile> (trm.Const c) :: t" and "E \<turnstile> (trm.Var xa) :: t"
+    by cases
+  from Eq_Var2(4)  have "x = xa" by auto
+  from this `E \<turnstile> (trm.Var xa) :: t` have "E x = t" using  wty_trm.cases by fastforce
+  from this Eq_Var2 ` E \<turnstile> (trm.Const c) :: t` show ?case
+    by (metis \<open>x = xa\<close> empty_iff eval_trm'.simps(1) fvi_trm.simps(2) sat'.simps(3) eval_trm_sound ty_of_eval_trm)
+  
+next
+  case (neq_Var xa)
+  thus ?case by (auto) 
+next
+  case (Pred p tms)
+  from Pred.prems(1) obtain tys where
+    S_p: "S p = Some tys" and
+    xs_ts: "list_all2 (\<lambda>tm ty. E \<turnstile> tm :: ty) tms tys"
+    by cases
+  let ?xs = "map (eval_trm' v) tms"
+  have wty_xs: "wty_tuple tys ?xs"
+  proof (cases "p \<in> dom V")
+    case True
+    then have "?xs \<in> the (V p) i"
+      using Pred.prems(3) by auto
+    with True show ?thesis
+      using Pred.prems(2) by (auto simp: S_p dest!: wty_envs_V_D)
+  next
+    case False
+    then have "(p, ?xs) \<in> \<Gamma> \<sigma> i"
+      using Pred.prems(3) by (auto split: option.splits)
+    with False show ?thesis
+      using Pred.prems(2) by (auto simp: S_p dest!: wty_envs_\<Gamma>_D)
+  qed
+  from Pred obtain k where k: "k < length tms" "tms ! k = Formula.Var x"
+    by (fastforce simp: trm.is_Var_def trm.is_Const_def in_set_conv_nth)
+  with Pred.prems have "v ! x = ?xs ! k" by simp
+  with wty_xs k have "ty_of (v ! x) = tys ! k"
+    by (auto simp: wty_tuple_def list_all2_conv_all_nth)
+  also have "\<dots> = E x"
+    using xs_ts k
+    by (fastforce simp: list_all2_conv_all_nth elim: wty_trm.cases)
+  finally show ?case .
+next
+  case (Let p \<phi> \<psi>)
+  let ?V' = "V(p \<mapsto> \<lambda>i. {v. length v = Formula.nfv \<phi> \<and> sat' \<sigma> V v i \<phi>})"
+  from Let.prems(1) obtain E' where
+    wty_\<phi>: "S, E' \<turnstile> \<phi>" and
+    wty_\<psi>: "S(p \<mapsto> tabulate E' 0 (Formula.nfv \<phi>)), E \<turnstile> \<psi>"
+    by (cases pred: wty_formula)
+  let ?tys = "tabulate E' 0 (Formula.nfv \<phi>)"
+  {
+    fix v' i
+    assume "length v' = Formula.nfv \<phi>" and "sat' \<sigma> V v' i \<phi>"
+    then have "wty_tuple ?tys v'"
+      using Let.IH(1) wty_\<phi> Let.prems(2) Let.hyps(1)
+      by (auto simp: wty_tuple_def list_all2_conv_all_nth)
+  }
+  with Let.prems(2) have "wty_envs (S(p \<mapsto> ?tys)) \<sigma> ?V'"
+    by (auto simp: wty_envs_def wty_event_def)
+  from Let.prems(3) have "sat' \<sigma> ?V' v i \<psi>" by simp
+  from Let.prems(4) have "x \<in> fv \<psi>" by simp
+  from Let have "Formula.nfv \<psi> \<le> length v" by auto
+  show ?case by (rule Let.IH(2)) fact+
+next
+  case (And_assign \<phi> \<psi>)
+  from And_assign.prems(1) have phi1: "S, E \<turnstile> \<phi>" by cases
+  from And_assign.prems(3) have phi2: "sat' \<sigma> V v i \<psi>" by auto
+  from And_assign.prems(4) have "x \<in> fv \<phi> \<or> x \<in> fv \<psi>" by auto
+  from this show ?case
+  proof cases
+    assume "x \<in> fv \<phi>"
+    from this And_assign phi1 phi2 show ?case by auto
+  next
+    assume x_not_\<phi>: "x \<notin> fv \<phi>"
+    from this And_assign.prems(4) have "x \<in> fv \<psi>" by auto
+    from And_assign.hyps(2) obtain a b where \<psi>_eq: "\<psi> = Formula.Eq a b"
+      by (auto simp: safe_assignment_def split: formula.splits)
+    moreover {
+      assume a_def: "a = Formula.Var x"
+      from this  x_not_\<phi> have fvb: "fv_trm b \<subseteq> fv \<phi>" using And_assign(2) by  (auto simp: safe_assignment_def \<psi>_eq split: trm.splits) 
+      have eval:" v! x = eval_trm' v b" using And_assign(6) a_def \<psi>_eq by auto
+      have Ebx: "E \<turnstile> b :: E  x"  using And_assign(4) by (auto simp: \<psi>_eq a_def elim: wty_trm.cases wty_formula.cases)
+      have "(\<lambda>y. ty_of (v ! y)) \<turnstile> b :: E x" apply (rule  iffD1[OF wty_trm_fv_cong,OF _ Ebx]) apply (subst eq_commute) 
+        apply (rule And_assign(3)) using And_assign fvb by (auto elim: wty_formula.cases) 
+      then have ?case using ty_of_eval_trm unfolding eval
+        using And_assign(4) by (auto simp: \<psi>_eq a_def eval_trm_sound elim: wty_formula.cases)
+    }
+    moreover {
+     assume a_def: "b = Formula.Var x"
+      from this  x_not_\<phi> have fvb: "fv_trm a \<subseteq> fv \<phi>" using And_assign(2) by  (auto simp: safe_assignment_def \<psi>_eq split: trm.splits) 
+      have eval:" v! x = eval_trm' v a" using And_assign(6) a_def \<psi>_eq by auto
+      have Ebx: "E \<turnstile> a :: E  x"  using And_assign(4) by (auto simp: \<psi>_eq a_def elim: wty_trm.cases wty_formula.cases)
+      have "(\<lambda>y. ty_of (v ! y)) \<turnstile> a :: E x" apply (rule  iffD1[OF wty_trm_fv_cong,OF _ Ebx]) apply (subst eq_commute) 
+        apply (rule And_assign(3)) using And_assign fvb by (auto elim: wty_formula.cases) 
+      then have ?case using ty_of_eval_trm unfolding eval
+        using And_assign(4)  by (auto simp: \<psi>_eq a_def eval_trm_sound elim: wty_formula.cases)
+    }
+    moreover
+      have "a = Formula.Var x \<or> b = Formula.Var x" using And_assign(2) And_assign(7) x_not_\<phi> by (auto simp: \<psi>_eq safe_assignment_def split: Formula.trm.splits) 
+    ultimately show ?case by auto
+qed
+ next
+  case (And_safe \<phi> \<psi>)
+  from And_safe.prems(1) obtain "S, E \<turnstile> \<phi>" and "S, E \<turnstile> \<psi>" by cases
+  from And_safe.prems(3) have "sat' \<sigma> V v i \<phi>" and "sat' \<sigma> V v i \<psi>"
+    by simp_all
+  from And_safe.prems(4) consider (in_\<phi>) "x \<in> fv \<phi>" | (in_\<psi>) "x \<in> fv \<psi>" by auto
+  then show ?case
+  proof cases
+    case in_\<phi>
+  from And_safe have "Formula.nfv \<phi> \<le> length v" by auto
+    show ?thesis by (rule And_safe.IH(1)) fact+
+  next
+    case in_\<psi>
+  from And_safe have "Formula.nfv \<psi> \<le> length v" by auto
+    show ?thesis by (rule And_safe.IH(2)) fact+
+  qed
+next
+  case (And_constraint \<phi> \<psi>)
+  have xfree: "x \<in> fv \<phi>" using And_constraint(4) And_constraint(10) by auto
+  from And_constraint(7) have "S, E \<turnstile> \<phi>" by cases
+  from this xfree And_constraint(6,8-9,11) show ?case by auto
+next
+  case (And_Not \<phi> \<psi>)
+  from And_Not.prems(4) And_Not.hyps(4) have xfree: "x \<in> fv \<phi>" by auto
+  from And_Not.prems(1) have "S, E \<turnstile> \<phi>" by cases
+  from this xfree And_Not  show ?case by auto 
+next
+  case (Ands l pos neg)
+  from Ands have "\<exists>\<phi> \<in> set l . x \<in> fv \<phi>" by auto
+  from this obtain \<psi> where psidef: "\<psi> \<in> set l \<and> x \<in> fv \<psi>" by blast
+  from this have "\<exists>\<phi>\<in>set pos. x \<in>fv  \<phi>" 
+  proof cases
+    assume "safe_formula \<psi>"
+    then have "\<psi> \<in> set pos" using Ands(1) by (auto simp add: psidef)
+    thus "\<exists>\<phi>\<in>set pos. x \<in>fv  \<phi>" using psidef by auto
+  next
+    assume " \<not> safe_formula \<psi>"
+    then have "\<psi> \<in> set neg" using Ands(1) by (auto simp add: psidef)
+    thus "\<exists>\<phi>\<in>set pos. x \<in>fv  \<phi>" using Ands(1) Ands(5) psidef by auto
+  qed
+  from this obtain \<phi> where phidef: "\<phi> \<in> set pos \<and> x \<in> fv \<phi>" by blast
+  from this Ands(1) have phi_in_l: "\<phi> \<in> set l" by auto
+  from phidef Ands(6) have phi_IH: "S, E \<turnstile> \<phi> \<Longrightarrow>
+    wty_envs S \<sigma> V \<Longrightarrow>
+    sat' \<sigma> V v i \<phi> \<Longrightarrow> x \<in> fv \<phi> \<Longrightarrow> Formula.nfv \<phi> \<le> length v \<Longrightarrow> ty_of (v ! x) = E x"
+        using list_all2_iff by (smt (verit, ccfv_SIG) Ball_set_list_all)
+      from Ands.prems(1) have  "\<forall>\<phi> \<in> set l. S, E \<turnstile> \<phi>" by cases
+      from this phi_in_l have p1: "S, E \<turnstile> \<phi>"  by auto
+      from phi_in_l Ands.prems(3) have p3: "sat' \<sigma> V v i \<phi>" by auto
+      from phi_in_l Ands have p5: "Formula.nfv \<phi> \<le> length v" by auto
+  from  phi_IH p1 Ands.prems(2) p3 phidef p5  show ?case by auto
+next
+  case (Neg \<phi>)
+  from Neg show ?case by auto
+next
+  case (Or \<phi> \<psi>)
+  from Or.prems(3) have " (sat' \<sigma> V v i \<phi>) \<or>( sat' \<sigma> V v i \<psi>)" by auto
+  from this show ?case 
+  proof
+    assume assm: "(sat' \<sigma> V v i \<phi>)"
+  from Or(1) Or.prems(4) have xfv: "x \<in> fv \<phi>" by auto
+  from Or.prems(1) have "S, E \<turnstile> \<phi>" by cases
+  from this assm Or.prems(2,3) Or(4) Or.prems(5) xfv show ?case by auto
+next 
+  assume assm: "( sat' \<sigma> V v i \<psi>)"
+ from Or(1) Or.prems(4) have xfv: "x \<in> fv \<psi>" by auto
+  from Or.prems(1) have "S, E \<turnstile> \<psi>" by cases
+  from this assm Or.prems(2,3) Or(5) Or.prems(5) xfv show ?case by auto
+qed
+next
+  case (Exists \<phi>)
+  from Exists.prems(1) obtain t where "S, case_nat t E \<turnstile> \<phi>" by cases
+  from Exists.prems(3) obtain z where "sat' \<sigma> V (z#v) i \<phi>" by auto
+  from Exists.prems(4) have "Suc x \<in> fv \<phi>" by (simp add: fvi_Suc)
+  from Exists have "Formula.nfv \<phi> \<le> Suc (length v)" apply (auto simp add: Formula.nfv_def)
+    by (metis fvi_Suc le0 old.nat.exhaust)
+
+  have "ty_of ((z#v) ! Suc x) = case_nat t E (Suc x)"
+    by (rule Exists.IH) (simp?, fact)+
+  then show ?case by simp
+next
+  case (Agg y \<omega> tys f \<phi>)
+ have "\<forall>z \<in>Formula.fvi (length tys) \<phi>. Suc z \<le> length v " using Agg.prems(5) by (auto simp add: Formula.nfv_def)
+    from this have "\<forall>z \<in>Formula.fv \<phi>. Suc z - length tys \<le> length v "  using  fvi_iff_fv  nat_le_linear 
+      by (metis Suc_diff_le diff_add diff_is_0_eq' diff_zero not_less_eq_eq) 
+    from this have nfv_tys_v: "Formula.nfv \<phi> \<le> length tys + length v" by (auto simp add: Formula.nfv_def)
+
+  have case_split:" x \<in> Formula.fvi (length tys) \<phi> \<or> x \<in> Formula.fvi_trm (length tys) f \<or> x = y" using Agg.prems(4) by auto
+ 
+  moreover {
+    assume asm: "x \<in> Formula.fvi (length tys) \<phi>"
+    from this have "\<not> fv \<phi> \<subseteq> {0..< length tys}" using fvi_iff_fv[of x "length tys" \<phi>] by auto
+    from this have M: "{(x, ecard Zs) | 
+  x Zs. Zs = {zs. length zs = length tys \<and> sat' \<sigma> V (zs @ v) i \<phi> \<and> eval_trm' (zs @ v) f = x} \<and> Zs \<noteq> {}} \<noteq> {}" using Agg.prems(3) by auto
+    from this obtain zs where sat: "sat' \<sigma> V (zs @ v) i \<phi> \<and> length zs = length tys" by auto
+    from nfv_tys_v have nfv: "Formula.nfv \<phi> \<le> length (zs @ v)"  by (auto simp add: sat)
+    have "ty_of ((zs@v) ! (x + length tys)) = agg_env E tys (x + length tys)"
+      apply (rule Agg.IH[of \<phi> S "agg_env E tys" V "zs @ v" i "x+ length tys"]) using Agg.prems(1) Agg(4) sat asm nfv Agg.prems(1-2) fvi_iff_fv
+      by (auto elim: wty_formula.cases)
+    from this have ?case apply (auto simp add: agg_env_def) by (metis add.commute nth_append_length_plus sat)
+  } 
+  moreover {
+    assume "x \<notin> Formula.fvi (length tys) \<phi>"
+    from this have eq: "x = y" using Agg(3) case_split fvi_iff_fv fvi_trm_iff_fv_trm by blast
+    obtain d agg_type where omega_def: "\<omega> = (agg_type, d)" using surjective_pairing by blast
+    from Agg.prems(1) this have  "\<exists>t .E y = t_res agg_type t" by cases auto
+    from this eq obtain t where t_def: "E x = t_res agg_type t" by blast
+    from  Agg.prems(1) have
+ ty_of_d: "ty_of d = t_res agg_type t" apply cases using eq omega_def t_def by auto
+    from Agg.prems(3) eq obtain M where  M_def: "M = {(x, ecard Zs) | x Zs. Zs = {zs. length zs = length tys \<and> sat' \<sigma> V (zs @ v) i \<phi>
+        \<and> eval_trm' (zs @ v) f = x} \<and> Zs \<noteq> {}} \<and> v!x = eval_agg_op' \<omega> M" by auto
+   
+        {
+           assume finite_M: "finite_multiset M"
+    from this   have finite_set:"finite {x. {zs. length zs = length tys \<and> sat' \<sigma> V (zs @ v) i \<phi> \<and> eval_trm' (zs @ v) f = x} \<noteq> {}}"
+       using finite_fst by (auto simp add: finite_multiset_def M_def ) 
+    have flatten: "set (flatten_multiset M) \<subseteq> fst ` M" using finite_set  set_of_flatten_multiset[of M
+ "(\<lambda>x . {zs . length zs = length tys \<and> sat' \<sigma> V (zs @ v) i \<phi> \<and> eval_trm' (zs @ v) f = x} )"]
+       by (auto simp add:  M_def) 
+    from this  have evaltrm: "z \<in> set (flatten_multiset M) \<Longrightarrow>  \<exists> zs. length zs = length tys \<and> sat' \<sigma> V (zs @ v) i \<phi> \<and> eval_trm' (zs @ v) f = z" 
+      for z using  M_def by (auto simp add: image_def)
+     have th2: ?case if minmaxsum: "agg_type = agg_type.Agg_Min \<or> agg_type = agg_type.Agg_Max \<or> agg_type = agg_type.Agg_Sum" and alist_def: " flatten_multiset
+     {(x, ecard {zs. length zs = length tys \<and> sat' \<sigma> V (zs @ v) i \<phi> \<and> eval_trm' (zs @ v) f = x}) |x.
+      \<exists>xa. sat' \<sigma> V (xa @ v) i \<phi> \<and> length xa = length tys \<and> eval_trm' (xa @ v) f = x} =
+    a # list"  for a list
+     proof -
+      have ty_of_list: "z=a \<or> z \<in> set list \<Longrightarrow> \<exists>zs .ty_of (eval_trm' (zs @ v) f) = t \<and> ty_of z = t" for z
+      proof -
+          assume z_def: "z=a \<or> z \<in> set list"
+        from z_def obtain zs where zs_def: " length zs = length tys \<and> sat' \<sigma> V (zs @ v) i \<phi> \<and> eval_trm' (zs @ v) f = z" using alist_def evaltrm M_def by auto
+        from Agg.prems(1) have wty_f: " agg_env E tys  \<turnstile> f :: t" apply cases  using omega_def t_def minmaxsum eq  by auto  
+        have fv_ty:"\<forall>y\<in>fv_trm f. ty_of ((zs @ v) ! y) = agg_env E tys y"
+        proof 
+          fix y
+          assume assm: "y \<in> fv_trm f"
+          have  sat: "sat' \<sigma> V (zs @ v) i \<phi>"  using zs_def by auto 
+          show "ty_of ((zs @ v) ! y) = agg_env E tys y" using zs_def assm Agg(3,4) Agg.prems(1-2) nfv_tys_v sat  Agg.IH[of \<phi> S "agg_env E tys" V "zs@v" i y]
+            by (auto elim: wty_formula.cases)
+        qed      
+        have ty_of_z: "ty_of (eval_trm' (zs @ v) f) = t" using wty_f fv_ty   ty_of_eval_trm[of "agg_env E tys" f t "zs@v" ]
+          by (auto simp add: eval_trm_sound)
+        from this zs_def show  ?thesis by auto
+      qed 
+      from this obtain zs where zs_def: "ty_of (eval_trm' (zs @ v) f) = t" by auto
+      from ty_of_list have indass: "ty_of a = t \<and> (\<forall>z \<in> set list . ty_of z = t)" by auto
+     
+      from this have foldl_evaltrm: "foldfun = min \<or> foldfun = max
+        \<Longrightarrow> ty_of (foldl foldfun a list) = ty_of (eval_trm' (zs @ v) f)" for foldfun using indass 
+          proof  (induction list arbitrary: a foldfun)
+            case Nil
+            then show ?case using zs_def by auto
+          next
+            case (Cons aa tail)
+             have minmax: " ty_of (foldl foldfun (foldfun a aa) tail) = ty_of (eval_trm' (zs @ v) f)"
+              using Cons.IH[of _ "foldfun a aa"] Cons apply auto 
+               apply (metis min_def) by (metis max_def) 
+              then show ?case by auto
+            qed
+
+          from indass have foldl_evaltrm_Sum: 
+              "t \<in> numeric_ty \<Longrightarrow> ty_of (foldl undef_plus a list) = ty_of (eval_trm' (zs@v) f)" 
+              proof (induction list arbitrary: a)
+                  case (Cons aa tail)
+                  from this have "ty_of (undef_plus a aa) = t"  apply (cases aa)  apply ( auto simp add: numeric_ty_def ty_of_plus)
+                     apply (cases a) apply (auto simp add: undef_plus_sound)
+                    by (cases a)(auto simp add: undef_plus_sound)
+
+                  then show ?case using Cons.prems(1) Cons.IH[of "undef_plus a aa"] apply auto 
+                    by (metis Cons.prems(2) list.set_intros(2))
+                qed (auto simp add: zs_def)
+
+ from indass have foldl_evaltrm_Min: 
+              " ty_of (foldl undef_min a list) = t" 
+              proof (induction list arbitrary: a)
+                  case (Cons aa tail)
+            from this have "ty_of (undef_min a aa) = t"  apply (cases aa) by ( auto simp add: numeric_ty_def undef_min_def undef_less_eq_sound)
+                  then show ?case using Cons.prems(1) Cons.IH[of "undef_min a aa"] by auto 
+                qed auto
+
+ from indass have foldl_evaltrm_Max: 
+              " ty_of (foldl undef_max a list) = t" 
+              proof (induction list arbitrary: a)
+                  case (Cons aa tail)
+            from this have "ty_of (undef_max a aa) = t"  apply (cases aa) by ( auto simp add: numeric_ty_def undef_max_def undef_less_eq_sound)
+                  then show ?case using Cons.prems(1) Cons.IH[of "undef_max a aa"] by auto 
+              qed auto
+           from Agg.prems(1) t_def eq omega_def have num_ty: "agg_type = agg_type.Agg_Sum \<Longrightarrow> t \<in> numeric_ty" by cases auto
+         
+    
+            from  num_ty  finite_M foldl_evaltrm foldl_evaltrm_Sum foldl_evaltrm_Min foldl_evaltrm_Max show  ?thesis apply (cases agg_type)
+               by (auto simp add: M_def  alist_def omega_def finite_multiset_def   
+                      t_def zs_def   split: list.splits) 
+   
+         qed
+          from  finite_M th2  M_def t_def omega_def  have ?case apply (cases agg_type) 
+            by (auto simp add: ty_of_d split: list.splits)        
+        }
+        moreover{
+             assume not_finite: "\<not> finite_multiset M"
+         from this t_def  M_def  omega_def have  ?case apply (cases agg_type)
+                by ( auto simp add: ty_of_d split: list.splits) 
+         }
+         ultimately have ?case by auto 
+     
+  } 
+  ultimately show ?case by auto
+next
+  
+  case (Prev I \<phi>)
+   from Prev.prems(1) have wty: "S, E \<turnstile> \<phi>" by cases
+  from Prev.prems(3) have forall_j: "\<forall>j . i = Suc j \<longrightarrow> sat' \<sigma> V v j \<phi>" by auto
+  from this have "sat' \<sigma> V v (Nat.pred i) \<phi>" using Prev.prems by (auto split: nat.splits)
+  from this wty Prev.prems(2-5) Prev.IH show ?case by auto
+next
+  case (Next I \<phi>)
+  from Next.prems(1,2-5) Next.IH show ?case by (auto elim: wty_formula.cases)
+next
+  case (Since \<phi> I \<psi>)
+  from Since(1,9) have xfv: "x \<in> fv \<psi>" by auto
+  from this  Since.prems(1,2-5) Since.IH show ?case by (auto elim: wty_formula.cases)
+next
+  case (Not_Since \<phi> I \<psi>)
+  from Not_Since.prems(1) have wty: "S, E \<turnstile> \<psi>" by cases
+  from Not_Since(1,10) have xfv: "x \<in> fv \<psi>" by auto
+  from this wty Not_Since.prems(2-5) Not_Since.IH show ?case by auto
+next
+  case (Until \<phi> I \<psi>)
+  from Until(1,9) have xfv: "x \<in> fv \<psi>" by auto
+  from this  Until.prems(1,2-5) Until.IH show ?case by (auto elim: wty_formula.cases)
+next
+  case (Not_Until \<phi> I \<psi>)
+ from Not_Until.prems(1) have wty: "S, E \<turnstile> \<psi>" by cases
+  from Not_Until(1,10) have xfv: "x \<in> fv \<psi>" by auto
+  from this wty Not_Until.prems(2-5) Not_Until.IH show ?case by auto
+next
+  case (MatchP I r)
+  from MatchP.prems(3) have "(\<exists>j. Regex.match (sat' \<sigma> V v) r j i)" by auto
+    from this  MatchP(1)  MatchP.prems(4) obtain \<phi> j where phidef: " \<phi> \<in> atms r" " sat' \<sigma> V v j \<phi>" "x \<in> fv \<phi> " using match_sat'_fv  by auto blast
+    have "\<forall>a \<in> fv \<phi>. a \<in> fv_regex r" using   phidef(1)  apply (induction r) apply auto 
+      subgoal for \<psi>  apply (cases "safe_formula \<psi>") apply auto by (cases \<psi>) auto 
+      done
+    from  this MatchP.prems(4,5) phidef  have nfv: "Formula.nfv \<phi> \<le> length v"  by  (auto simp add: Formula.nfv_def)
+    from MatchP.IH MatchP.prems have IH: "S, E \<turnstile> \<phi> \<Longrightarrow>\<phi> \<in> atms r \<Longrightarrow>
+     sat' \<sigma> V v j \<phi> \<Longrightarrow> x \<in> fv \<phi> \<Longrightarrow> Formula.nfv \<phi> \<le> length v \<Longrightarrow> ty_of (v ! x ) = E x"
+    for \<phi> E  v  x by blast
+   from MatchP.prems(1) MatchP(1) have  "S, E \<turnstile> \<phi>" using  Regex.Regex.regex.pred_set[of "(\<lambda>\<phi>. S, E \<turnstile> \<phi>)"] phidef(1) wty_regexatms_atms  by cases auto
+  then show ?case apply (rule IH) using nfv  MatchP.prems(5) phidef by auto
+ 
+next
+  case (MatchF I r)
+ from MatchF.prems(3) have "(\<exists>j. Regex.match (sat' \<sigma> V v) r  i j)" by auto
+    from this  MatchF(1)  MatchF.prems(4) obtain \<phi> j where phidef: " \<phi> \<in> atms r" " sat' \<sigma> V v j \<phi>" "x \<in> fv \<phi> " using match_sat'_fv  by auto blast
+    have "\<forall>a \<in> fv \<phi>. a \<in> fv_regex r" using   phidef(1)  apply (induction r) apply auto 
+      subgoal for \<psi>  apply (cases "safe_formula \<psi>") apply auto by (cases \<psi>) auto 
+      done
+    from  this MatchF.prems(4,5) phidef  have nfv: "Formula.nfv \<phi> \<le> length v"  by  (auto simp add: Formula.nfv_def)
+    from MatchF.IH MatchF.prems have IH: "S, E \<turnstile> \<phi> \<Longrightarrow>\<phi> \<in> atms r \<Longrightarrow>
+     sat' \<sigma> V v j \<phi> \<Longrightarrow> x \<in> fv \<phi> \<Longrightarrow> Formula.nfv \<phi> \<le> length v \<Longrightarrow> ty_of (v ! x ) = E x"
+    for \<phi> E  v  x by blast
+    from MatchF.prems(1) MatchF(1) have  "S, E \<turnstile> \<phi>" using  Regex.Regex.regex.pred_set[of "(\<lambda>\<phi>. S, E \<turnstile> \<phi>)"] phidef(1) wty_regexatms_atms  by cases auto
+  then show ?case apply (rule IH) using nfv  MatchF.prems(5)  phidef by auto
+
+qed
+
 
 lemma soundness:
   assumes  "S,E \<turnstile> \<phi>" "\<forall>y\<in>fv \<phi>. ty_of (v ! y) = E y" "safe_formula \<phi>" "wty_envs S \<sigma> V"
@@ -205,8 +612,8 @@ next
    assume  assm: "local.sat' \<sigma> V (za # v) i \<phi>" 
  have nfv: " Formula.nfv \<phi> \<le> Suc (length v)" using Exists(6) nfv_exists[of \<phi> t] by auto
     have "0 \<in> fv \<phi> \<Longrightarrow> ty_of za = t" 
-      using ty_of_sat_safe[where ?E="case_nat t E" and ?S=S and ?\<phi>=\<phi> and ?v="za#v" and ?V=V and ?i=i and ?\<sigma>=\<sigma> and ?x=0]  
-      Exists(1,4-5)  nfv assm apply auto sorry
+      using ty_of_sat'_safe[where ?E="case_nat t E" and ?S=S and ?\<phi>=\<phi> and ?v="za#v" and ?V=V and ?i=i and ?\<sigma>=\<sigma> and ?x=0]  
+      Exists(1,4-5)  nfv assm by auto
     from this have "\<forall>y\<in>fv \<phi>. ty_of ((za # v) ! y) = (case y of 0 \<Rightarrow> t | Suc x \<Rightarrow> E x)" using Exists(3) assm by (auto simp add: fvi_Suc split: nat.splits )
     from this have " Formula.sat \<sigma> V (za # v) i \<phi>" using Exists.IH[of "za#v" V i] Exists(4-6) nfv_exists[of \<phi> t] assm by auto
   }
@@ -214,7 +621,7 @@ next
 next
   case (MatchF S E x2 x1) 
   from this  have other_IH: "\<phi> \<in> regex.atms x2 \<Longrightarrow> Formula.sat \<sigma> V5 v i5 \<phi> = local.sat' \<sigma> V5 v i5 \<phi>" for \<phi> V5 i5 
-    using MatchF by (auto simp add: regex.pred_set fv_regex_alt) 
+    using MatchF apply (auto simp add: regex.pred_set fv_regex_alt) 
   then show ?case  using match_cong[OF refl other_IH, where ?r=x2] by auto 
 next
   case (MatchP S E x2 x1)
@@ -222,6 +629,8 @@ next
     by (auto simp add: regex.pred_set fv_regex_alt)
   then show ?case  using match_cong[OF refl other_IH, where ?r=x2] by auto 
 qed  (auto split: nat.splits) 
+  oops
+
 
 end
 end
